APM1111 - Formative Assessment 2
================
Dacanay, Jordan
2024-09-10

**3.49** Prove that $$
\sum_{j=1}^{N}(X_{j}-1)^{2}=\sum_{j=1}^{N}X_{j}^{2}-2\sum_{j=1}^{N}X_{j}+N
$$ **Proof**:

Expanding the left-hand side: $$
\sum_{j=1}^{N}(X_{j}-1)^{2}
$$ Expanding the square inside the summation: $$
(X_{j}-1)^{2}=X_{j}^2-2X_{j}+1
$$ Therefore, the summation becomes: $$
\sum_{j=1}^{N}(X_{j}-1)^{2}=\sum_{j=1}^{N}(X_{j}^2-2X_{j}+1)
$$ Distributing the summation: $$
\sum_{j=1}^{N}(X_{j}^2-2X_{j}+1) = \sum_{j=1}^{N}X_{j}^2 - 2\sum_{j=1}^{N}X_{j} + \sum_{j=1}^{N}1
$$ Since $$
\sum_{j=1}^{N}1 = N
$$ Therefore, the equation will become $$
\sum_{j=1}^{N}(X_{j}^2-2X_{j}+1) = \sum_{j=1}^{N}X_{j}^2 - 2\sum_{j=1}^{N}X_{j} + N
$$ Thus, we have proven the equation. ∎

:::

**3.51** Two variables, U and V, assume the values $$
U_1=3,\ U_2=-2,\ U_3=5,\ and\\ V_1=4,\ V_2=-1,\ V_3=6 
$$ **Calculate (a)** $$
\sum UV
$$ Given that there are three U values and V values, we can expand the
equation: $$
\sum UV = \sum_i^NU_iV_i
$$ Substituting the value i and N: $$
\sum_i^NU_iV_i = \sum_1^3U_iV_i = U_1V_1 + U_2V_2 + U_3V_3
$$ Substituting the given values: $$
U_1V_1 + U_2V_2 + U_3V_3 = 3(-4)+(-2)(-1)+5(6)
$$ Simplifying this: $$
−12+2+30=20
$$ Therefore, $$
\sum UV = 20
$$ **Calculate (b)** $$
\sum(U+3)(V-4)
$$ Expanding the equation: $$
\sum(U+3)(V-4) = \sum_1^3(U_i+3)(V_i-4) = (U_1+3)(V_1-4) + (U_2+3)(V_2-4) + (U_3+3)(V_3-4)
$$ Substituting the values: $$
(U_1+3)(V_1-4) + (U_2+3)(V_2-4) + (U_3+3)(V_3-4) = (3+3)(-4-4)+(-2+3)(-1-4)+(5+3)(6-4)
$$ Simplifying this: $$
6(-8)+1(-5)+8(2)=-24+(-4)+16=36
$$ Therefore, $$
\sum(U+3)(V-4) = 36
$$ **Calculate (c)** $$
\sum V^2
$$ Expanding the equation: $$
\sum V^2 = \sum_1^3 V_i^2 = V_1^2+V_2^2+V_3^2
$$ Substituting the values: $$
V_1^2+V_2^2+V_3^2 = (-4)^2+(-1)^2+6^2
$$ Simplifying this: $$
16+1+36=53
$$ Therefore, $$
\sum V^2 = 53
$$ **Calculate (d)** $$
(\sum U)(\sum V)^2
$$ Expanding the equation: $$
(\sum U)(\sum V)^2 = (\sum_1^3 U_i)(\sum_1^3 V_i)^2 = [U_1+U_2+U_3][V_1+V_2+V_3]^2
$$ Substituting the values: $$
[U_1+U_2+U_3][V_1+V_2+V_3]^2 = [3+(-2)+5][-4+(-1)+6]^2
$$ Simplifying this: $$
6(1)^2 = 6
$$ Therefore, $$
(\sum U)(\sum V)^2 = 6
$$ **Calculate (e)** $$
\sum UV^2
$$ Expanding the equation: $$
\sum UV^2 = \sum_1^3U_iV_i^2 = U_1V_1^2 + U_2V_2^2 + U_3V_3^2
$$ Substituting the values: $$
U_1V_1^2 + U_2V_2^2 + U_3V_3^2 = 3(-4)^2 + (-2)(-1)^2+5(6)^2
$$ Simplifying this: $$
3(-4)^2 + (-2)(-1)^2+5(6)^2 = 48+(-2)+41 = 87
$$ Therefore, $$
\sum UV^2 = 87
$$ **Calculate (f)** $$
\sum (U^2-2V^2+2)
$$ Expanding the equation: $$
\sum (U^2-2V^2+2) = \sum_1^3 U_i^2 - 2\sum_1^3 V_i^2 + \sum_1^32) = (U_1^2+U_2^2+U_3^2)-2(V_1^2+V_2^2+V_3^2)+2N
$$ Substituting the values: $$
(U_1^2+U_2^2+U_3^2)-2(V_1^2+V_2^2+V_3^2)+2N = (3^2+(-2)^2+5^2) - 2((-4)^2+(-1)^2+6^2) + 2(3)
$$ Simplifying this: $$
(9+4+25)-2(16+1+36)+6 = 38-2(53)+6 = 38-106+6 = -62
$$ Therefore, $$
\sum (U^2-2V^2+2) = 62
$$ **Calculate (g)** $$
\sum (U/V)
$$ Expanding the equation: $$
\sum (U/V) = \frac{\sum_1^3 U_i}{\sum_1^3 V_i}=\frac{U_1+U_2+U_3}{V_1+V_2+V_3}
$$ Substituting the values: $$
\frac{U_1+U_2+U_3}{V_1+V_2+V_3} = \frac{3+(-2)+5}{-4-1-6}
$$ Simplifying this: $$
\frac{6}{-11}
$$ Therefore, $$
\sum (U/V) = \frac{6}{-11}
$$
